getting stuck due to non-informative error or not typechecking conditions

share/pulse/examples/dice/dpe/SPDM3.fst
@@ -55,6 +55,7 @@ let init_inv (key_len:u32) (b:Seq.seq u8) (s:state) (r:gref) : slprop =
 
 let pcm_elt (p:perm) (t:trace) : pcm_t = Some p, t
 
+
 fn init0 (key_size:u32) (signing_pub_key:V.vec u8 { V.length signing_pub_key == U32.v key_size })
   (#p:perm)
   (#s:Seq.seq u8)
@@ -64,14 +65,143 @@ fn init0 (key_size:u32) (signing_pub_key:V.vec u8 { V.length signing_pub_key == 
           init_inv key_size s (fst r) (snd r)
 {
   let session_transcript = V.alloc 0uy 0sz;
-  let c_st = Initialized { key_size; signing_pub_key; session_transcript };
   
-  let tr_elt = G_Initialized ({key_size_repr = key_size; signing_pub_key_repr = s; transcript = Seq.empty});
-  let trace = next_trace emp_trace tr_elt;
-  let r = ghost_alloc #trace_pcm_t #trace_pcm (pcm_elt 1.0R trace);
+  //prove this assumption
+  _assume ((Seq.Base.create (SZ.v 0sz) 0uy) == Seq.empty);
 
-  admit ()
+  let st_repr = { key_size; signing_pub_key; session_transcript };
+  let c_st = Initialized st_repr;
+  
+  let repr = {key_size_repr = key_size; signing_pub_key_repr = s; transcript = Seq.empty};
+  
+  let tr_elt = G_Initialized repr;
+  let trace = next_trace emp_trace tr_elt;
+  
+  let r = ghost_alloc #trace_pcm_t #trace_pcm (pcm_elt 1.0R trace);
+  
+ (*Current context:
+    ghost_pcm_pts_to r (G.reveal (G.hide (pcm_elt 1.0R trace))) **
+    V.pts_to session_transcript (Seq.Base.create (SZ.v 0sz) 0uy) **
+    V.pts_to signing_pub_key s*)
+
+  
+  with _v. rewrite  (ghost_pcm_pts_to r (G.reveal (G.hide _v))) as 
+                     (ghost_pcm_pts_to r _v);
+  assert (pure (st_repr.key_size == repr.key_size_repr));
+  assert (V.pts_to session_transcript (Seq.Base.create (SZ.v 0sz) 0uy));
+
+  rewrite each
+    signing_pub_key  as st_repr.signing_pub_key,
+    session_transcript as st_repr.session_transcript; 
+  
+  rewrite each 
+  s as repr.signing_pub_key_repr;
+  
+  rewrite each 
+  (Seq.Base.create (SZ.v 0sz) 0uy) as Seq.empty #u8;
+
+  assert (pure (c_st == Initialized st_repr));
+  assert (pure (tr_elt == G_Initialized repr));
+  assert (pure (current_state trace == G_Initialized repr));
+  assert (V.pts_to st_repr.session_transcript Seq.Base.empty);
+  assert (pure (st_repr.key_size == repr.key_size_repr));
+  (*-----------------------------------------------------------------------------------*)
+  (*CONTEXT HAS THIS CONDITION, THEN WHY THE BELOW ASSERT IS NOT PASSING?*)
+  (*How can I add an assume, adding __assume with this condition shows some type error.*)
+  (*-----------------------------------------------------------------------------------*)
+  //assert ( V.pts_to st_repr.signing_pub_key repr.signing_pub_key_repr); //NEED TO UNDERSTAND THIS.
+  (*Current context:
+    ghost_pcm_pts_to r (pcm_elt 1.0R trace) **
+    V.pts_to st_repr.session_transcript Seq.Base.empty **
+    V.pts_to st_repr.signing_pub_key repr.signing_pub_key_repr*)
+  
+  match c_st {
+    Initialized st_repr -> {
+      //What is going wrong here? Why it is not typechecking or not showing errors?
+      //Plan is to say unreachable in all branches except the G_Initialized
+      show_proof_state;
+       (*match (current_state trace){
+        G_UnInitialized  -> {
+          admit()
+        }
+        G_Initialized _ -> {
+          admit()
+        }
+        G_Recv_no_sign_resp _ -> {
+          admit()
+        }
+        G_Recv_sign_resp _ -> {
+          admit()
+        }
+       }*)
+      
+
+     }
+    
+     Recv_no_sign_resp st_repr -> {
+      
+      unreachable ()
+     }
+  }
+  
+(* G_UnInitialized ->{
+        admit()
+      }
+      G_Initialized k ->{
+        admit()
+      }
+      G_Recv_no_sign_resp  _ -> {
+        admit()
+      }
+      G_Recv_sign_resp _ -> {
+        admit()
+      }*)
+
+  (*(SPDM3.Initialized st)
+      (SPDM3.G_Initialized repr) ->
+      (V.pts_to st.signing_pub_key repr.signing_pub_key_repr **
+      V.pts_to st.session_transcript Seq.Base.empty) **
+      pure (st.key_size == repr.key_size_repr)*)
+  
+  (* ghost_pcm_pts_to r (pcm_elt 1.0R trace) **
+    V.pts_to st_repr.session_transcript Seq.Base.empty **
+    V.pts_to st_repr.signing_pub_key repr.signing_pub_key_repr*)
+
+  (*To prove,
+    exists* (t:trace).
+    spdm_inv s r t ** 
+    pure (G_Initialized? (current_state t) /\
+          g_key_of_gst (current_state t) == b /\
+          g_key_len_of_gst (current_state t) == key_len)*)
+  
 }
+
+(*rewrite each
+        ctr as (fst ret).st_ctr,
+        tbl as (fst ret).st_tbl;*)
+
+
+(*fold (dpe_inv r None);*)
+
+(*let spdm_inv (s:state) (r:gref) (t:trace) : slprop =
+  ghost_pcm_pts_to r (Some 1.0R, t) **
+  session_state_related s (current_state t)*)
+
+(*let session_state_related (s:state) (gs:g_state) : slprop =
+  match s, gs with
+  | Initialized st, G_Initialized repr ->
+    V.pts_to st.signing_pub_key repr.signing_pub_key_repr **
+    V.pts_to st.session_transcript Seq.empty **
+    pure (st.key_size == repr.key_size_repr)
+
+  | Recv_no_sign_resp st, G_Recv_no_sign_resp repr ->
+    V.pts_to st.signing_pub_key repr.signing_pub_key_repr **
+    V.pts_to st.session_transcript repr.transcript **
+    pure (st.key_size == repr.key_size_repr)
+
+  | _ -> pure False
+
+//*)
 
 
 // We assume a combinator to run pulse computations for initialization of top-level state, it gets primitive support in extraction
@@ -80,7 +210,7 @@ assume val run_stt (#a:Type) (#post:a -> slprop) (f:stt a emp post) : a
 // We assume this code will be executed on a machine where u32 fits the word size
 assume SZ_fits_u32 : SZ.fits_u32
 
-let trace_ref : gref = admit()
+
 
 fn __init (s:state) (t:trace) (key_len:u32) (signing_key:V.vec u8 { V.length signing_key == U32.v key_len})
   requires spdm_inv s trace_ref t
@@ -97,7 +227,7 @@ assume val emptyVector : v:V.vec u8{V.length v = 0}
  //how to bring in init_client_perm r b key_len?
  //how to bring in b? That is the seq version of signing_key
 
-fn init  (key_len:u32) (signing_key:V.vec u8 { V.length signing_key == U32.v key_len })
+fn init1  (key_len:u32) (signing_key:V.vec u8 { V.length signing_key == U32.v key_len })
   requires (exists* p b. V.pts_to signing_key #p b)
   returns r:(state)
   ensures (exists* p b. V.pts_to signing_key #p b ** 
